Created method for representing natural numbers via gates from BooleanCompilation

VOQC/src/BooleanCompilation.v
@@ -1,5 +1,5 @@
-Require Import UnitaryOps.
-Open Scope ucom.
+Require Import  UnitaryOps.
+Local Open Scope ucom.
 
 (*********************************)
 (** Boolean Circuit Compilation **)
@@ -26,7 +26,10 @@ Inductive bexp :=
 | b_f   : bexp
 | b_var : nat -> bexp
 | b_and : bexp -> bexp -> bexp 
-| b_xor : bexp -> bexp -> bexp.
+| b_xor : bexp -> bexp -> bexp
+| b_or : bexp -> bexp -> bexp
+| b_not : bexp -> bexp.
+
 
 Fixpoint interpret_bexp (b : bexp) (f : nat -> bool) : bool :=
   match b with
@@ -35,27 +38,55 @@ Fixpoint interpret_bexp (b : bexp) (f : nat -> bool) : bool :=
   | b_var v     => f v 
   | b_and b1 b2 => (interpret_bexp b1 f) && (interpret_bexp b2 f)
   | b_xor b1 b2 => (interpret_bexp b1 f) ⊕ (interpret_bexp b2 f)
+  | b_or b1 b2 => (interpret_bexp b1 f) || (interpret_bexp b2 f)
+  | b_not b1 => negb (interpret_bexp b1 f)
   end.  
+
 
 Inductive bexp_well_typed : nat -> bexp -> Prop :=
   | WT_b_t : forall n, bexp_well_typed n b_t
   | WT_b_f : forall n, bexp_well_typed n b_f
   | WT_b_var : forall n q, (q < n)%nat -> bexp_well_typed n (b_var q)
   | WT_b_and : forall n b1 b2, bexp_well_typed n b1 -> bexp_well_typed n b2 -> bexp_well_typed n (b_and b1 b2)
-  | WT_b_xor : forall n b1 b2, bexp_well_typed n b1 -> bexp_well_typed n b2 -> bexp_well_typed n (b_xor b1 b2).
-
+  | WT_b_xor : forall n b1 b2, bexp_well_typed n b1 -> bexp_well_typed n b2 -> bexp_well_typed n (b_xor b1 b2)
+  | WT_b_or : forall n b1 b2, bexp_well_typed n b1 -> bexp_well_typed n b2 -> bexp_well_typed n (b_or b1 b2) 
+  | WT_b_not : forall n b1, bexp_well_typed n b1 -> bexp_well_typed n (b_not b1).
+    
 Lemma well_typed_increase_dim : forall b n n',
   (n <= n')%nat ->
   bexp_well_typed n b ->
   bexp_well_typed n' b.
 Proof.
   intros.
-  induction H0; try constructor; try lia;
+  induction H0.
+  - try constructor; try lia;
   try apply IHbexp_well_typed1; 
   try apply IHbexp_well_typed2; 
   assumption.
+  - try constructor; try lia;
+  try apply IHbexp_well_typed1; 
+  try apply IHbexp_well_typed2; 
+  assumption.
+  - try constructor; try lia;
+  try apply IHbexp_well_typed1; 
+  try apply IHbexp_well_typed2; 
+  assumption.
+  - try constructor; try lia;
+  try apply IHbexp_well_typed1; 
+  try apply IHbexp_well_typed2; 
+  assumption.
+  - try constructor. try lia.
+  try apply IHbexp_well_typed1; 
+  try apply IHbexp_well_typed2; 
+  assumption. try lia. try apply IHbexp_well_typed1. try apply IHbexp_well_typed2. assumption.
+  - try constructor. try lia.
+    try apply IHbexp_well_typed1;
+      try apply IHbexp_well_typed2;
+      assumption. try lia. try apply IHbexp_well_typed1. try apply IHbexp_well_typed2. assumption.
+  - try constructor. try lia.
+  try apply IHbexp_well_typed.
+  assumption.
 Qed.
-
 Lemma interpret_bexp_f : forall i b f f',
   bexp_well_typed i b ->
   (forall k, (k < i)%nat -> f k = f' k) ->
@@ -69,6 +100,11 @@ Proof.
     reflexivity.
   - rewrite IHbexp_well_typed1; try assumption.
     rewrite IHbexp_well_typed2; try assumption.
+    reflexivity.
+  - rewrite IHbexp_well_typed1; try assumption.
+    rewrite IHbexp_well_typed2; try assumption.
+    reflexivity.
+  - rewrite IHbexp_well_typed; try assumption.
     reflexivity.
 Qed.
 
@@ -84,6 +120,7 @@ Proof.
   reflexivity.
 Qed.
 
+
 (** Compilation of boolean expressions to oracles **)
 
 (* How many input variables does this expression use? *)
@@ -92,6 +129,8 @@ Fixpoint max_var b v :=
   | b_var v' => max v v'
   | b_and b1 b2 => max (max_var b1 v) (max_var b2 v)
   | b_xor b1 b2 => max (max_var b1 v) (max_var b2 v)
+  | b_or b1 b2 => max (max_var b1 v) (max_var b2 v)
+  | b_not b1 => max_var b1 v
   | _ => v
   end.
 
@@ -100,11 +139,12 @@ Fixpoint no_vars b :=
   | b_var _ => false
   | b_and b1 b2 => no_vars b1 && no_vars b2
   | b_xor b1 b2 => no_vars b1 && no_vars b2
+  | b_or b1 b2 => no_vars b1 && no_vars b2
+  | b_not b1 => no_vars b1
   | _ => true
   end.
 
 Definition num_inputs b : nat := if (no_vars b) then 0 else (max_var b 0) + 1.
-
 Lemma num_inputs_well_typed : forall b,
   bexp_well_typed (num_inputs b) b.
 Proof.
@@ -127,13 +167,26 @@ Proof.
     + apply well_typed_increase_dim with (n:=num_inputs b2); try assumption.
       unfold num_inputs.
       simpl; destruct (no_vars b1); destruct (no_vars b2); simpl; lia.
+  - constructor.
+    + apply well_typed_increase_dim with (n:=num_inputs b1); try assumption.
+      unfold num_inputs.
+      simpl; destruct (no_vars b1); destruct (no_vars b2); simpl; lia.
+    + apply well_typed_increase_dim with (n:=num_inputs b2); try assumption.
+      unfold num_inputs.
+      simpl; destruct (no_vars b1); destruct (no_vars b2); simpl; lia.
+  - constructor.
+    + apply well_typed_increase_dim with (n:=num_inputs b); try assumption.
+      unfold num_inputs.
+      simpl; lia.
 Qed.
 
 (* How many ancillary qubits are needed to represent this expression? *)
 Fixpoint num_ancillae b : nat :=
   match b with
   | b_and b1 b2 => 2 + (max (num_ancillae b1) (num_ancillae b2))
-  | b_xor b1 b2 => max (num_ancillae b1) (num_ancillae b2) 
+  | b_xor b1 b2 => max (num_ancillae b1) (num_ancillae b2)
+  | b_not b1 => 1 + num_ancillae b1
+  | b_or b1 b2 => 2 + (max (num_ancillae b1) (num_ancillae b2))
   | _ => 0
   end.
 
@@ -156,7 +209,18 @@ Fixpoint compile' {dim} (b : bexp) (i j : nat) : base_ucom dim :=
                   compile' b1 j (j+2)
   | b_xor b1 b2 => compile' b1 i j; 
                   compile' b2 i j
+  | b_or b1 b2 => compile' b1 j (j + 2);
+                  compile' b2 (j+1) (j + 2);
+                 CCX  j (j+1) i;
+                compile' b2 (j+1) (j +2 );
+                  compile' b1 j (j + 2);
+                  compile' b1 i (j + 2);
+                  compile' b2 i (j + 2)
+  
+         
+  | b_not b1    => compile' b1 i j; X i        
   end.
+
 
 Definition compile b : base_ucom (b_dim b) := 
   compile' b (num_inputs b) ((num_inputs b) + 1).
@@ -172,6 +236,15 @@ Definition compile b : base_ucom (b_dim b) :=
      case -- note that this is the only case where the ancilla matter.
 *)
 Local Opaque CCX.
+
+Lemma and_xor_or : forall ( a b : bool),
+    (a && b) ⊕ (a ⊕ b) = (a || b).
+Proof.
+  intros.
+  induction a.
+  -rewrite orb_true_l. rewrite andb_true_l. rewrite xorb_true_l. rewrite <- negb_xorb_r. rewrite xorb_nilpotent. rewrite negb_true_iff. reflexivity.
+  -rewrite orb_false_l. rewrite andb_false_l. rewrite xorb_false_l. rewrite xorb_false_l. reflexivity. Qed.
+
 Lemma compile'_correct : forall dim (b : bexp) (f : nat -> bool) (i j : nat),
   bexp_well_typed i b -> 
   (i < j)%nat ->
@@ -273,7 +346,97 @@ Proof.
       try assumption; try lia.
     rewrite xorb_assoc.
     reflexivity.
-Qed.
+    - (* b_or b1 b2 *) (*This contains the proof for b_and- I'm not sure of a way to extract that from both of them into a lemma that's applied twice *) 
+    inversion H; subst; clear H.
+    assert (bexp_well_typed j b1).
+    { apply (well_typed_increase_dim b1 i j); try assumption; lia. }
+     assert (bexp_well_typed (j+1) b2).
+    { apply (well_typed_increase_dim b2 i (j+1)); try assumption; lia. }
+    assert (j < j + 2)%nat by lia.
+    assert (j + 1 < j + 2)%nat by lia.
+    simpl in H1.
+    assert ((j + 2) + num_ancillae b1 < dim + 1)%nat by lia.
+    assert ((j + 2) + num_ancillae b2 < dim + 1)%nat by lia.
+    assert(IHb3 := IHb1).
+    assert(IHb4 := IHb2).
+    assert(i < j + 2)%nat by lia.
+    specialize (IHb4 i H7 (j+2)%nat H10 H9).
+    specialize (IHb3 i H6 (j+2)%nat H10 H8).
+    specialize (IHb1 j H (j+2)%nat H4 H8).
+    specialize (IHb2 (j+1)%nat H3 (j+2)%nat H5 H9).
+    clear H H3 H4 H5 H8 H9.
+    simpl.
+    repeat rewrite Mmult_assoc.
+    rewrite IHb1.
+    2: { intros. apply H2. lia. }
+    rewrite IHb2.
+    2: { intros. rewrite update_index_neq; try apply H2; lia. }
+    rewrite update_index_neq; try lia.
+    rewrite <- interpret_bexp_update with (i:=i);
+      try assumption; try lia.
+    rewrite f_to_vec_CCX; try lia.
+    rewrite update_index_eq. 
+    do 3 (rewrite update_index_neq; try lia).
+    rewrite update_index_eq.
+    rewrite IHb2.
+    2: { intros. repeat rewrite update_index_neq; try apply H2; lia. }
+    rewrite (update_twice_neq _ (j+1)); try lia.
+    rewrite update_twice_eq. 
+    rewrite update_index_eq.
+    repeat rewrite <- interpret_bexp_update with (i:=i);
+      try assumption; try lia.
+    rewrite xorb_assoc.
+    rewrite xorb_nilpotent.
+    rewrite xorb_false_r.
+    rewrite IHb1.
+    2: { intros. 
+         rewrite update_twice_neq; try lia.
+         rewrite update_index_neq; try lia.
+         rewrite update_twice_neq; try lia.
+         rewrite update_index_neq; try lia.
+         rewrite update_same; try reflexivity.
+         apply H2; lia. }
+    do 2 (rewrite (update_twice_neq _ j); try lia).
+    rewrite update_twice_eq.
+    rewrite update_index_eq.
+    repeat rewrite <- interpret_bexp_update with (i:=i);
+      try assumption; try lia.
+    rewrite xorb_assoc.
+    rewrite xorb_nilpotent.
+    rewrite xorb_false_r.
+    repeat rewrite (update_twice_neq _ i); try lia.
+    rewrite (update_same _ (j+1)); try reflexivity.
+    rewrite (update_same _ j); try reflexivity.
+    rewrite H2 with (k:=j); try lia.
+    rewrite H2 with (k:=(j+1)%nat); try lia.
+    repeat rewrite xorb_false_l.
+    simpl.
+    rewrite IHb3.
+    rewrite IHb4.
+        rewrite update_twice_eq.
+    rewrite update_index_eq.
+    rewrite <- interpret_bexp_update with (i:=i);
+      try assumption; try lia.
+    rewrite xorb_assoc.
+    repeat rewrite update_index_eq.
+    repeat rewrite update_twice_eq.
+    rewrite xorb_assoc.
+    rewrite <- interpret_bexp_update with (i:=i);
+      try assumption; try lia.
+    rewrite and_xor_or. reflexivity.
+     +intros. assert (i <> k)%nat by lia. rewrite update_index_eq. rewrite update_twice_eq. repeat rewrite update_twice_eq. rewrite update_index_neq. apply H2. apply H. apply H3.
+     +intros. assert (i <> k)%nat by lia. rewrite update_index_neq. apply H2. apply H. apply H3.
+      (*- b_not b1 *)
+  - inversion H. subst. clear H.
+    simpl.
+    rewrite Mmult_assoc.
+    simpl in H1. repeat rewrite Mmult_assoc.
+    rewrite IHb; try assumption; try lia.
+    rewrite f_to_vec_X; try lia. 
+    rewrite update_index_eq.
+    rewrite update_twice_eq; try lia.
+    rewrite <- negb_xorb_r.
+    reflexivity. Qed.
 
 Lemma compile_correct : forall (b : bexp) (f : nat -> bool) (r : bool), 
   let in_s := fun i => if i <? (num_inputs b) then f i else false in
@@ -325,6 +488,9 @@ Input : var 0 : y
         var 2 : cin
 Output : sum = cin ⊕ (x ⊕ y)
  *)
+Definition xor_test : bexp := (b_t ⊻ b_t).
+Eval cbv in (compile xor_test).
+
 Definition adder_sum_bexp : bexp := 2 ⊻ (1 ⊻ 0).
 Eval cbv in (compile adder_sum_bexp).
 
